coq/theories/fp2imp/FpToImpCodegenProof.v
@@ -1,0 +1,566 @@
+Require Import impboot.utils.Core.
+Require Import impboot.functional.FunSyntax.
+Require Import impboot.functional.FunSemantics.
+Require Import impboot.functional.FunValues.
+Require Import impboot.imperative.ImpSyntax.
+Require Import impboot.imperative.ImpSemantics.
+Require Import impboot.imperative.ImpProperties.
+Require Import coqutil.Word.Interface.
+Require Import coqutil.Word.Properties.
+Require Import impboot.fp2imp.FpToImpCodegen.
+Require Import impboot.commons.ProofUtils.
+Require Import Stdlib.Program.Equality.
+
+Require Import Patat.Patat.
+
+Open Scope N.
+
+Fixpoint list_rel {A} {B} (R: A -> B -> Prop) (al: list A) (bl: list B): Prop :=
+  match al, bl with
+  | nil, nil => True
+  | a :: al, b :: bl => R a b /\ list_rel R al bl
+  | _, _ => False
+  end.
+
+Inductive v_rel: list mem_block -> FunValues.Value -> ImpSyntax.Value -> Prop :=
+| v_Num (n: N) (mem: list mem_block)
+  (N_IN_BOUNDS: n < 2^64):
+    v_rel mem (Num n) (Word (word.of_Z (Z.of_N n)))
+| v_Pair (p: nat) (mem: list mem_block) (v1 v2: FunValues.Value) (w1 w2: Value)
+  (MEM_AT_P: nth_error mem p = Some [Some w1; Some w2])
+  (v1_rel: v_rel mem v1 w1) (v2_rel: v_rel mem v2 w2):
+    v_rel mem (Pair v1 v2) (Pointer p).
+
+Definition func_rel (s: list defun) (t: list func) :=
+  (∀ n ps cs, In (n, ps, cs) builtin -> find_fun n t = Some (ps,cs)) ∧
+  ∀ fname params body,
+    lookup_fun fname s = Some (params,body) ->
+    ∃ cs, find_fun fname t = Some (params,cs) ∧
+      to_cmd body = Some cs ∧ NoDup params.
+
+Definition state_rel (s: FunSemantics.state) (t: ImpSemantics.state) :=
+  t.(input) = s.(FunSemantics.input) ∧
+  t.(output) = s.(FunSemantics.output) ∧
+  func_rel s.(FunSemantics.funs) t.(funs).
+
+Definition env_rel (mem: list mem_block) (s_env: FEnv.env) (t_env: IEnv.env) :=
+  ∀n v,
+    FEnv.lookup s_env n = Some v ->
+    ∃w, IEnv.lookup t_env n = Some w ∧ v_rel mem v w.
+
+Definition res_rel (mem: list mem_block) (v: FunValues.Value) (o: outcome unit) (s: FunSemantics.state) (t: ImpSemantics.state): Prop :=
+  match o with
+  | (Stop (Return w)) => 
+    v_rel mem v w ∧
+      state_rel s t
+  | (Stop Abort) => True
+  | _ => False
+  end.
+
+Fixpoint mem_prefix (m1 m2: list mem_block): Prop :=
+  match m1, m2 with
+  | [], _ => True
+  | b1 :: m1', b2 :: m2' => b1 = b2 ∧ mem_prefix m1' m2'
+  | _, _ => False
+  end.
+
+Lemma mem_prefix_refl: ∀m, mem_prefix m m.
+Proof.
+  induction m; simpl; eauto.
+Qed.
+
+Lemma mem_prefix_trans: ∀m1 m2 m3,
+  mem_prefix m1 m2 -> mem_prefix m2 m3 -> mem_prefix m1 m3.
+Proof.
+  induction m1; intros * Hprefix1 Hprefix2; simpl in *; cleanup; eauto.
+  destruct m2; simpl in *; try discriminate; cleanup.
+  destruct m3; simpl in *; try discriminate; cleanup.
+  subst; eauto.
+Qed.
+
+Opaque word.of_Z Nat.div Nat.modulo Z.to_nat.
+
+Theorem to_exps_thm: ∀ (es: list FunSyntax.exp) (s: FunSemantics.state) (t: ImpSemantics.state)
+  (env: FEnv.env) (vs: list FunValues.Value) (s1: FunSemantics.state)
+  (Heval: env |-- (es, s) ---> (vs, s1)),
+  ∀ (xs: list ImpSyntax.exp)
+    (Hto_exp: to_exps es = Some xs)
+    (Hstate_rel: state_rel s t)
+    (Henv_rel: env_rel t.(memory) env t.(vars)),
+    ∃ (ws: list ImpSyntax.Value),
+      eval_exps xs t = ((Cont ws), t) ∧ s = s1 ∧ list_rel (v_rel t.(memory)) vs ws.
+Proof.
+  intros * Heval.
+  induction Heval; intros; simpl in *; unfold option_bind in *; cleanup.
+  - (* Nil *)
+    exists []; split; [reflexivity|].
+    eauto.
+  - (* Cons *)
+    repeat (pat `match ?vs with _ => _ end = _` at destruct vs eqn:?); simpl in *; unfold fail in *; unfold return_ in *; cleanup.
+    assert (Some [e] = Some [e]) as HeqSome by congruence.
+    eapply IHHeval1 in HeqSome; eauto; clear IHHeval1; cleanup; subst.
+    assert (Some (e0 :: l0) = Some (e0 :: l0)) as HeqSome by congruence.
+    eapply IHHeval2 in HeqSome; eauto; clear IHHeval2.
+    simpl in *; unfold bind in *.
+    repeat (spat `match ?vs with _ => _ end` at destruct vs eqn:?); simpl in *; cleanup; unfold_outcome; subst; cleanup.
+    eexists.
+    spat `eval_exp e0` at rewrite spat.
+    spat `eval_exps l0` at rewrite spat.
+    eauto.
+  - (* Const *)
+    destruct (_ <? _) eqn:Hlt; rewrite ?N.ltb_lt in *; inversion Hto_exp; subst.
+    eexists.
+    split; [reflexivity|].
+    split; [reflexivity|].
+    split; eauto.
+    econstructor; simpl; eauto.
+  - (* Var *)
+    unfold env_rel in Henv_rel; specialize Henv_rel with (1:= ENV_LOOKUP); destruct Henv_rel as [w [Hlookup Hvr]].
+    eexists; simpl; unfold lookup_var, bind; rewrite Hlookup; unfold_outcome.
+    eauto.
+  - (* Op *)
+    destruct op; try solve [inversion Hto_exp]; destruct exps; try solve [inversion Hto_exp]; destruct exps; try solve [inversion Hto_exp].
+    + (* Head *)
+      inversion EVAL_OP; subst; simpl in *; unfold option_bind in *; cleanup.
+      repeat (pat `match ?vs with _ => _ end = _` at destruct vs eqn:?); simpl in *; unfold fail in *; unfold return_ in *; cleanup.
+      destruct to_exp eqn:Hto_expeq; try discriminate; simpl in *; cleanup.
+      assert (Some [e1] = Some [e1]) as HSomeeq by reflexivity.
+      eapply IHHeval in HSomeeq; eauto; clear IHHeval; cleanup; subst; simpl in *; unfold bind in *; cleanup.
+      repeat (pat `match ?vs with _ => _ end = _` at destruct vs eqn:?); simpl in *; unfold fail in *; unfold return_ in *; unfold_outcome; cleanup.
+      destruct mem_load eqn:Hmem_load.
+      spat `v_rel` at inversion spat; subst.
+      unfold_monadic; unfold w2n in *; rewrite Properties.word.unsigned_of_Z_0 in *; simpl in *; rewrite Nat.Div0.mod_0_l in *; simpl in *.
+      spat `nth_error` at rewrite spat in *; rewrite Nat.Div0.div_0_l in *; simpl in *; unfold_outcome; cleanup.
+      eexists; eauto.
+    + (* Tail *)
+      inversion EVAL_OP; subst; simpl in *; unfold option_bind in *; cleanup.
+      repeat (pat `match ?vs with _ => _ end = _` at destruct vs eqn:?); simpl in *; unfold fail in *; unfold return_ in *; cleanup.
+      destruct to_exp eqn:Hto_expeq; try discriminate; simpl in *; cleanup.
+      assert (Some [e1] = Some [e1]) as HSomeeq by reflexivity.
+      eapply IHHeval in HSomeeq; eauto; clear IHHeval; cleanup; subst; simpl in *; unfold bind in *; cleanup.
+      repeat (pat `match ?vs with _ => _ end = _` at destruct vs eqn:?); simpl in *; unfold fail in *; unfold return_ in *; unfold_outcome; cleanup.
+      destruct mem_load eqn:Hmem_load.
+      spat `v_rel` at inversion spat; subst.
+      unfold_monadic; unfold w2n in *; rewrite Properties.word.unsigned_of_Z_nowrap in *; try lia; simpl in *; rewrite Nat.Div0.mod_same in *; simpl in *.
+      assert (Z.to_nat 8 = 8%nat) as Htmp by lia; rewrite Htmp in *; clear Htmp.
+      spat `nth_error` at rewrite spat in *; rewrite Nat.div_same in *; try lia; simpl in *; unfold_outcome; cleanup.
+      eexists; eauto.
+Admitted. (* Cannot Qed? *)
+
+Theorem to_exp_thm: ∀ (e: FunSyntax.exp) (s: FunSemantics.state) (t: ImpSemantics.state)
+  (env: FEnv.env) (v: FunValues.Value) (s1: FunSemantics.state)
+  (Heval: env |-- ([e], s) ---> ([v], s1)),
+  ∀ (x: ImpSyntax.exp)
+    (Hto_exp: to_exp e = Some x)
+    (Hstate_rel: state_rel s t)
+    (Henv_rel: env_rel t.(memory) env t.(vars)),
+    ∃ (w: ImpSyntax.Value),
+      eval_exp x t = ((Cont w), t) ∧ s = s1 ∧ v_rel t.(memory) v w.
+Proof.
+  intros.
+  specialize to_exps_thm with (Heval := Heval) (es := [e]) (xs := [x]) (Hstate_rel := Hstate_rel) (Henv_rel := Henv_rel) as Hto_exps.
+  simpl to_exps in *; unfold option_bind in *; cleanup.
+  rewrite Hto_exp in Hto_exps.
+  specialize Hto_exps with (1 := eq_refl); cleanup; subst.
+  simpl in *; unfold_monadic.
+  destruct eval_exp eqn:?; destruct o eqn:?; cleanup.
+  eauto.
+Qed.
+
+Lemma list_rel_length_same : forall [A B] (R: A -> B -> Prop) l l1,
+  list_rel R l l1 -> List.length l = List.length l1.
+Proof.
+  induction l; intros; simpl in *; eauto; cleanup.
+  all: destruct l1; simpl in *; cleanup; eauto.
+Qed.
+
+Theorem Eval_length:
+  ∀env es s rs s1,
+    env |-- (es, s) ---> (rs,s1) -> List.length es = List.length rs.
+Proof.
+  induction es; intros * Heval; simpl in *; inversion Heval; subst; simpl; eauto.
+Qed.
+
+Theorem env_rel_update: ∀ m env vars n v1 w,
+  env_rel m env vars -> v_rel m v1 w ->
+  env_rel m (FEnv.insert (n, Some v1) env) (IEnv.insert (n, Some w) vars).
+Proof.
+  intros * Henv_rel Hvr n0 v Hlookup.
+  destruct (N.eq_dec n0 n); subst; simpl.
+  - rewrite FEnv.lookup_insert_eq in *; cleanup.
+    eexists; split; eauto.
+    rewrite IEnv.lookup_insert_eq; reflexivity.
+  - rewrite FEnv.lookup_insert_neq in *; eauto; cleanup.
+    unfold env_rel in *; eauto; specialize Henv_rel with (1:= Hlookup); eauto; cleanup.
+    eexists; rewrite IEnv.lookup_insert_neq; eauto.
+Qed.
+
+(* Theorem oEL_isPREFIX:
+  ∀xs ys n, prefix xs ys = true -> (n < String.length xs)%nat -> substring 0 n xs = substring 0 n ys.
+Proof.
+Admitted.
+  (* Induct \\ Cases_on ‘ys’ \\ fs [oEL_def] \\ rw [] *)
+(* QED *)
+
+Theorem v_rel_isPREFIX:
+  ∀m v w, v_rel m v w -> ∀m', prefix m m' = true -> v_rel m' v w.
+Proof.
+  (* Induct_on ‘v_rel’ \\ rw []
+  \\ simp [Once v_rel_cases] \\ gvs []
+  \\ drule_all oEL_isPREFIX \\ rw [] *)
+(* QED *)
+
+Theorem env_rel_isPREFIX:
+  env_rel m1 env vars ∧ prefix m1 m2 = true -> env_rel m2 env vars.
+Proof.
+  (* rw [env_rel_def] \\ res_tac \\ fs []
+  \\ drule_all v_rel_isPREFIX \\ fs [] *)
+(* QED *)
+ *)
+
+Theorem env_rel_make_env: forall (rs: list FunValues.Value) ws params m,
+  list_rel (v_rel m) rs ws -> List.length params = List.length ws ->
+  env_rel m (FunSemantics.make_env params rs FEnv.empty) (make_env params ws IEnv.empty).
+Proof.
+Admitted.
+  (* fs [env_rel_def,PULL_FORALL,AND_IMP_INTRO] \\ rw []
+  \\ qsuff_tac ‘
+    ∀rs ws params m1 m2.
+       LIST_REL (v_rel m) rs ws ∧
+       LENGTH params = LENGTH ws ∧
+       (∀n v1. m1 n = SOME v1 -> ∃v2. FLOOKUP m2 n = SOME v2 ∧ v_rel m v1 v2) ∧
+       make_env params rs m1 n = SOME v ->
+       ∃w. FLOOKUP (m2 |++ ZIP (params,ws)) n = SOME w ∧ v_rel m v w’
+  >-
+   (disch_then irule \\ fs []
+    \\ rpt $ first_x_assum $ irule_at Any
+    \\ fs [empty_env_def])
+  \\ rpt $ pop_assum kall_tac
+  \\ Induct \\ fs [make_env_def,PULL_EXISTS,FUPDATE_LIST]
+  \\ gen_tac \\ Cases \\ fs [] \\ rw []
+  \\ fs [make_env_def]
+  \\ last_x_assum $ drule_at $ Pos last
+  \\ disch_then drule \\ fs []
+  \\ disch_then irule
+  \\ gvs [APPLY_UPDATE_THM,FLOOKUP_UPDATE]
+  \\ rw [] \\ fs [] *)
+(* QED *)
+
+Lemma state_rel_set_vars: ∀s t vars
+  (Hstate_rel: state_rel s t),
+  state_rel s (set_vars vars t).
+Proof.
+  unfold state_rel; intros; cleanup; eauto.
+Qed.
+
+Lemma func_rel_from_state_rel: ∀s t,
+  state_rel s t -> func_rel s.(FunSemantics.funs) t.(funs).
+Proof.
+  unfold state_rel; intros; cleanup; eauto.
+Qed.
+
+Lemma mem_prefix_nth_error: ∀m1 m2 p b
+  (Hmem_prefix: mem_prefix m1 m2)
+  (Hnth: nth_error m1 p = Some b),
+  nth_error m2 p = Some b.
+Proof.
+  induction m1; simpl; intros.
+  - rewrite nth_error_nil in *; discriminate.
+  - destruct m2; simpl in *; try discriminate; cleanup; subst.
+    destruct p; simpl in *; eauto.
+Qed.
+
+Lemma v_rel_mem_prefix: ∀m1 m2 v w
+  (Hv_rel: v_rel m1 v w)
+  (Hmem_prefix: mem_prefix m1 m2),
+  v_rel m2 v w.
+Proof.
+  intros * Hv_rel; induction Hv_rel; simpl; intros; subst.
+  - econstructor; eauto.
+  - econstructor; eauto.
+    eapply mem_prefix_nth_error; eauto.
+Qed.
+
+Lemma env_rel_mem_prefix: ∀m1 m2 env vars
+  (Henv_rel: env_rel m1 env vars)
+  (Hmem_prefix: mem_prefix m1 m2),
+  env_rel m2 env vars.
+Proof.
+  unfold env_rel; intros; cleanup.
+  specialize Henv_rel with (1:= H); cleanup.
+  eapply v_rel_mem_prefix in Hmem_prefix; eauto.
+Qed.
+
+Theorem to_cmd_thm: ∀ es env s rs s1
+  (Heval: env |-- (es, s) ---> (rs, s1)),
+  ∀ e cs t r,
+    es = [e] -> rs = [r] -> to_cmd e = Some cs -> state_rel s t ->
+    env_rel t.(memory) env t.(vars) ->
+    ∃ fuel r1 t1,
+      eval_cmd cs (EVAL_CMD fuel) t = (r1,t1) ∧
+      res_rel t1.(memory) r r1 s1 t1 ∧ mem_prefix t.(memory) t1.(memory).
+Proof.
+  Opaque word.ltu word.eqb.
+  Opaque to_exp.
+  fix IH 6.
+  intros * Heval; destruct Heval; try discriminate; intros * Hes Hrs Hto_cmd Hstate_rel Henv_rel; simpl in *; subst; cleanup; simpl in *.
+  - (* Const *)
+    destruct to_exp eqn:Hto_exp; cleanup; simpl in *|-; unfold_monadic; unfold_outcome.
+    eapply to_exp_thm in Hto_exp; eauto; cleanup; subst; [|econstructor; eauto]; subst.
+    do 3 eexists.
+    simpl in *; unfold_monadic; rewrite H.
+    split; [reflexivity|].
+    split; [|apply mem_prefix_refl].
+    unfold res_rel; simpl; split; eauto.
+  - (* Var *)
+    destruct to_exp eqn:Hto_exp; try discriminate; cleanup.
+    eapply to_exp_thm in Hto_exp; eauto; cleanup; subst; [|econstructor; eauto].
+    eapply Henv_rel in ENV_LOOKUP; cleanup.
+    do 3 eexists.
+    simpl in *; unfold_monadic; unfold lookup_var; rewrite H; unfold_outcome.
+    split; [reflexivity|].
+    split; [|apply mem_prefix_refl].
+    unfold res_rel; simpl; split; eauto.
+  - (* Op *)
+    destruct to_exp eqn:Hto_exp; try discriminate; cleanup.
+    destruct op; try solve [inversion Hto_exp]; destruct exps; try solve [inversion Hto_exp]; destruct exps; try solve [inversion Hto_exp].
+    all: eexists.
+    all: inversion EVAL_OP; subst; simpl in *; unfold option_bind in *; cleanup.
+    all: repeat (pat `match ?vs with _ => _ end = _` at destruct vs eqn:?); simpl in *; unfold fail in *; unfold return_ in *; cleanup.
+    all: destruct to_exp eqn:Hto_expeq; try discriminate; simpl in *; cleanup.
+    all: eapply to_exp_thm in Hto_expeq; eauto; cleanup; subst; [|econstructor; eauto; econstructor]; subst.
+    all: simpl in *; unfold_monadic; unfold_outcome; rewrite H.
+    all: do 2 eexists.
+    all: split; [reflexivity|].
+    all: split; [|apply mem_prefix_refl].
+    all: unfold res_rel; simpl; split; eauto.
+  - (* Let *)
+    destruct to_exp eqn:Hto_exp; try discriminate; cleanup.
+    unfold option_bind in *; cleanup.
+    destruct to_assign eqn:Hto_assign; try discriminate; cleanup.
+    unfold to_assign in Hto_assign; cleanup.
+    destruct (to_exp exp1) eqn:Hto_exp1; cleanup.
+    1: { (* assign expr *)
+      eapply to_exp_thm in Hto_exp1; cleanup; eauto; simpl in *; cleanup; subst.
+      destruct (to_cmd exp2) eqn:Hto_cmd2; try discriminate; cleanup.
+      eapply IH with (t := set_vars _ t) in Hto_cmd2; cleanup; eauto; simpl in *; cleanup.
+      2: eapply env_rel_update; eauto.
+      unfold assign; unfold_monadic; unfold_outcome.
+      do 3 eexists.
+      rewrite H.
+      split; [eauto|].
+      split; [|assumption].
+      eauto.
+    }
+    destruct to_cons eqn:Hto_cons; cleanup.
+    1: { (* assign cons *)
+      unfold to_cons in *; cleanup.
+      admit.
+    }
+    destruct exp1; try discriminate; cleanup.
+    2: { (* call *)
+      destruct to_exps eqn:Hto_exps; try discriminate; cleanup.
+      inversion Heval1; subst.
+      eapply to_exps_thm in Hto_exps; eauto; cleanup; subst.
+      specialize list_rel_length_same with (1:= H1) as Hlen.
+      specialize Eval_length with (1 := EVAL_ARGS) as Hlen_eval.
+      destruct (to_cmd exp2) eqn:Hto_cmd2; try discriminate; cleanup.
+      unfold env_and_body in *; destruct lookup_fun as [ [fparams fbody] | ] eqn:Hlookup_fun; try discriminate; cleanup.
+      destruct (_ =? _)%nat eqn:Hlen_params; rewrite ?Nat.eqb_eq in *; try discriminate; cleanup.
+      simpl in *; cleanup; unfold_monadic; simpl; unfold_monadic; unfold_outcome.
+      unfold get_vars, get_body_and_set_vars, set_varsM, assign, catch_return, set_vars; simpl; unfold_outcome.
+      specialize func_rel_from_state_rel with (1:= Hstate_rel) as Hfunc_rel.
+      eapply Hfunc_rel in Hlookup_fun; cleanup; clear Hfunc_rel.
+      eapply IH with (t := set_vars _ (set_steps_done _ _)) in EVAL_BODY; eauto; cleanup; simpl in *; cleanup.
+      3: eapply env_rel_make_env; eauto; congruence.
+      2: eapply state_rel_set_vars; eauto.
+      pat `eval_cmd _ (EVAL_CMD ?f) (set_vars _ _) = _` at rename f into fuel0.
+      unfold res_rel in *|-; simpl in *; cleanup.
+      eapply env_rel_mem_prefix in Henv_rel; eauto.
+      destruct x2; cleanup; destruct v; cleanup; eauto.
+      2: { (* Abort *)
+        exists (S fuel0); do 2 eexists.
+        rewrite H.
+        rewrite H0.
+        spat `NoDup` at eapply nodup_fixed_point in spat; rewrite spat.
+        rewrite Hlen_params, Hlen; rewrite Nat.eqb_refl; simpl; unfold nodupb.
+        unfold_monadic; unfold_outcome; unfold set_vars, inc_steps_done, add_steps_done, set_steps_done in *; simpl in *.
+        rewrite H4; unfold res_rel in *|-; simpl in *; cleanup.
+        split; eauto; split; eauto; simpl; eauto.
+      }
+      eapply IH with (t := set_vars _ _) in Heval2; eauto; simpl in *; cleanup.
+      3: eapply env_rel_update; eauto.
+      2: eapply state_rel_set_vars; eauto.
+      exists (S (fuel0 + x1)); do 2 eexists.
+      Opaque EVAL_CMD.
+      rewrite H.
+      rewrite H0.
+      spat `NoDup` at eapply nodup_fixed_point in spat; rewrite spat.
+      rewrite Hlen_params, Hlen; rewrite Nat.eqb_refl; simpl; unfold nodupb.
+      with_strategy transparent [EVAL_CMD] simpl EVAL_CMD at 1.
+      unfold_monadic; unfold_outcome; unfold set_vars, inc_steps_done, add_steps_done, set_steps_done in *; simpl in *.
+      eapply eval_cmd_add_clock with (fuel1 := x1) in H4; try congruence.
+      rewrite H4; unfold res_rel in *|-; simpl in *; cleanup.
+      rewrite Nat.add_comm.
+      destruct x2; cleanup; destruct v0; cleanup; eauto.
+      all: eapply eval_cmd_add_clock with (fuel1 := (fuel0 + 1)%nat) in H8; try congruence.
+      all: rewrite Nat.add_assoc, Nat.add_1_r in H8.
+      all: split; eauto.
+      all: split; eauto.
+      all: unfold res_rel; simpl; eauto.
+      all: eapply mem_prefix_trans; eauto.
+    }
+    (* Op *)
+    destruct o eqn:?; cleanup.
+    1: { (* Add *)
+      destruct to_exps as [iargs|] eqn:Hto_exps; cleanup.
+      destruct iargs as [|iarg1 iargs]; cleanup.
+      destruct iargs as [|iarg2 iargs]; cleanup.
+      destruct iargs; cleanup.
+      destruct to_cmd eqn:?; cleanup.
+      inversion Heval1; cleanup; subst.
+      eapply to_exps_thm in Hto_exps; eauto; cleanup; subst.
+      Opaque eval_exps.
+      simpl in *; unfold_monadic; unfold fail in *.
+      destruct vs as [|varg1 vs]; cleanup.
+      destruct varg1 as [|narg1]; cleanup.
+      destruct vs as [|varg2 vs]; cleanup.
+      destruct varg2 as [|narg2]; cleanup.
+      destruct vs; unfold return_ in *; cleanup.
+      simpl in *; destruct x as [|warg1 x]; cleanup.
+      destruct x as [|warg2 x]; cleanup.
+      destruct x; cleanup.
+      do 3 eexists.
+      simpl in *; unfold_monadic; rewrite H.
+      unfold get_body_and_set_vars.
+      admit.
+    }
+    all: admit.
+  - (* If *)
+    destruct to_exp eqn:Hto_exp; try discriminate; cleanup.
+    unfold option_bind in *; cleanup.
+    destruct to_guard eqn:Hto_guard; try discriminate; cleanup.
+    destruct to_cmd eqn:Hto_cmd1; try discriminate; cleanup.
+    destruct (to_cmd expf) eqn:Hto_cmd2; try discriminate; cleanup.
+    unfold to_guard in Hto_guard; cleanup.
+    destruct to_exps as [conds_vs|] eqn:Hto_exps; try discriminate; cleanup.
+    destruct conds_vs as [|cond_v1 conds_vs1] eqn:?; try discriminate; simpl in *; cleanup.
+    destruct conds_vs1 as [|cond_v2 conds_vs1]; try discriminate; simpl in *; cleanup.
+    destruct conds_vs1; try discriminate; simpl in *; cleanup.
+    eapply to_exps_thm in Hto_exps; eauto; cleanup; subst.
+    specialize list_rel_length_same with (1:= H1) as Hlen.
+    specialize Eval_length with (1 := Heval1) as Hlen_eval.
+    Transparent eval_exps.
+    simpl in *; unfold_monadic; unfold_outcome.
+    destruct eval_exp eqn:?; destruct o eqn:?; cleanup; subst.
+    destruct (eval_exp cond_v2) eqn:?; destruct o eqn:?; cleanup; subst.
+    destruct vs as [|v1 vs]; try discriminate; cleanup.
+    destruct vs as [|v2 vs]; try discriminate; cleanup.
+    destruct vs; try discriminate; cleanup.
+    destruct exps as [|e1 exps]; try discriminate; cleanup.
+    destruct exps as [|e2 exps]; try discriminate; cleanup.
+    destruct exps; try discriminate; cleanup.
+    destruct b.
+    + (* then branch *)
+      eapply IH in Hto_cmd1; cleanup; eauto; simpl in *; cleanup.
+      destruct eval_cmp eqn:?; unfold eval_cmp in *; simpl in *; unfold_monadic; unfold_outcome.
+      destruct test eqn:?; simpl in *.
+      1: { (* Less *)
+        unfold take_branch in *; destruct v1; unfold_outcome; try discriminate; destruct v2; unfold_outcome; try discriminate; simpl in *; unfold return_ in *; cleanup; inversion H3; inversion H1; subst.
+        assert (Z.of_N n <? Z.of_N n0 = true)%Z as Hlt by (rewrite N.ltb_lt, Z.ltb_lt in *; rewrite <- N2Z.inj_lt; eauto); cleanup.
+        rewrite word.unsigned_ltu; try lia; do 2 (rewrite Properties.word.unsigned_of_Z_nowrap; try lia); rewrite Hlt.
+        do 3 eexists.
+        rewrite H.
+        split; [reflexivity|].
+        split; [|assumption].
+        eauto.
+      }
+      unfold take_branch in *; destruct v1; unfold_outcome; try discriminate; destruct v2; unfold_outcome; try discriminate; simpl in *; unfold return_ in *; cleanup; inversion H3; inversion H1; subst.
+      1: destruct n; try discriminate.
+      cleanup.
+      assert (Z.of_N n =? Z.of_N n0 = true)%Z as Hlt by (rewrite N.eqb_eq, Z.eqb_eq in *; subst; eauto).
+      rewrite word.unsigned_eqb; try lia; do 2 (rewrite Properties.word.unsigned_of_Z_nowrap; try lia); rewrite Hlt.
+      do 3 eexists.
+      rewrite H.
+      split; [reflexivity|].
+      split; [|assumption].
+      eauto.
+    + (* else branch *)
+      eapply IH in Hto_cmd2; cleanup; eauto; simpl in *; cleanup.
+      destruct eval_cmp eqn:?; unfold eval_cmp in *; simpl in *; unfold_monadic; unfold_outcome.
+      destruct test eqn:?; simpl in *.
+      1: { (* Less *)
+        unfold take_branch in *; destruct v1; unfold_outcome; try discriminate; destruct v2; unfold_outcome; try discriminate; simpl in *; unfold return_ in *; cleanup; inversion H3; inversion H1; subst.
+        assert (Z.of_N n <? Z.of_N n0 = false)%Z as Hlt by (rewrite N.ltb_ge, Z.ltb_ge in *; rewrite <- N2Z.inj_le; eauto); cleanup.
+        rewrite word.unsigned_ltu; try lia; do 2 (rewrite Properties.word.unsigned_of_Z_nowrap; try lia); rewrite Hlt.
+        do 3 eexists.
+        rewrite H.
+        split; [reflexivity|].
+        split; [|assumption].
+        eauto.
+      }
+      unfold take_branch in *; destruct v1; unfold_outcome; try discriminate; destruct v2; unfold_outcome; try discriminate; simpl in *; unfold return_ in *; cleanup; inversion H3; inversion H1; subst.
+      1: destruct n; try discriminate.
+      all: cleanup.
+      2: assert (Z.of_N n =? Z.of_N n0 = false)%Z as Hlt by (rewrite N.eqb_neq, Z.eqb_neq in *; rewrite N2Z.inj_iff; eauto).
+      2: rewrite word.unsigned_eqb; try lia; do 2 (rewrite Properties.word.unsigned_of_Z_nowrap; try lia); rewrite Hlt.
+      1: assert (Z.of_N 0 = 0%Z) as Htmp by lia; rewrite Htmp in *; clear Htmp.
+      1: rewrite word.unsigned_eqb in *; try lia; rewrite Properties.word.unsigned_of_Z_nowrap in *; try lia; simpl in *; cleanup.
+      all: do 3 eexists.
+      all: rewrite H.
+      all: split; [reflexivity|].
+      all: split; [|assumption].
+      all: eauto.
+    - (* Call *)
+      (* destruct to_exp eqn:Hto_exp; try discriminate; cleanup.
+      inversion Heval1; subst.
+      eapply to_exps_thm in Hto_exps; eauto; cleanup; subst.
+      specialize list_rel_length_same with (1:= H1) as Hlen.
+      specialize Eval_length with (1 := EVAL_ARGS) as Hlen_eval.
+      destruct (to_cmd exp2) eqn:Hto_cmd2; try discriminate; cleanup.
+      unfold env_and_body in *; destruct lookup_fun as [ [fparams fbody] | ] eqn:Hlookup_fun; try discriminate; cleanup.
+      destruct (_ =? _)%nat eqn:Hlen_params; rewrite ?Nat.eqb_eq in *; try discriminate; cleanup.
+      simpl in *; cleanup; unfold_monadic; simpl; unfold_monadic; unfold_outcome.
+      unfold get_vars, get_body_and_set_vars, set_varsM, assign, catch_return, set_vars; simpl; unfold_outcome.
+      specialize func_rel_from_state_rel with (1:= Hstate_rel) as Hfunc_rel.
+      eapply Hfunc_rel in Hlookup_fun; cleanup; clear Hfunc_rel.
+      eapply IH with (t := set_vars _ (set_steps_done _ _)) in EVAL_BODY; eauto; cleanup; simpl in *; cleanup.
+      3: eapply env_rel_make_env; eauto; congruence.
+      2: eapply state_rel_set_vars; eauto.
+      pat `eval_cmd _ (EVAL_CMD ?f) (set_vars _ _) = _` at rename f into fuel0.
+      unfold res_rel in *|-; simpl in *; cleanup.
+      eapply env_rel_mem_prefix in Henv_rel; eauto.
+      destruct x2; cleanup; destruct v; cleanup; eauto.
+      2: { (* Abort *)
+        exists (S fuel0); do 2 eexists.
+        rewrite H.
+        rewrite H0.
+        spat `NoDup` at eapply nodup_fixed_point in spat; rewrite spat.
+        rewrite Hlen_params, Hlen; rewrite Nat.eqb_refl; simpl; unfold nodupb.
+        unfold_monadic; unfold_outcome; unfold set_vars, inc_steps_done, add_steps_done, set_steps_done in *; simpl in *.
+        rewrite H4; unfold res_rel in *|-; simpl in *; cleanup.
+        split; eauto; split; eauto; simpl; eauto.
+      }
+      eapply IH with (t := set_vars _ _) in Heval2; eauto; simpl in *; cleanup.
+      3: eapply env_rel_update; eauto.
+      2: eapply state_rel_set_vars; eauto.
+      exists (S (fuel0 + x1)); do 2 eexists.
+      Opaque EVAL_CMD.
+      rewrite H.
+      rewrite H0.
+      spat `NoDup` at eapply nodup_fixed_point in spat; rewrite spat.
+      rewrite Hlen_params, Hlen; rewrite Nat.eqb_refl; simpl; unfold nodupb.
+      with_strategy transparent [EVAL_CMD] simpl EVAL_CMD at 1.
+      unfold_monadic; unfold_outcome; unfold set_vars, inc_steps_done, add_steps_done, set_steps_done in *; simpl in *.
+      eapply eval_cmd_add_clock with (fuel1 := x1) in H4; try congruence.
+      rewrite H4; unfold res_rel in *|-; simpl in *; cleanup.
+      rewrite Nat.add_comm.
+      destruct x2; cleanup; destruct v0; cleanup; eauto.
+      all: eapply eval_cmd_add_clock with (fuel1 := (fuel0 + 1)%nat) in H8; try congruence.
+      all: rewrite Nat.add_assoc, Nat.add_1_r in H8.
+      all: split; eauto.
+      all: split; eauto.
+      all: unfold res_rel; simpl; eauto.
+      all: eapply mem_prefix_trans; eauto. *)
+    admit.
+Admitted.
