coq/theories/imp2asm/Compiler.v
@@ -1,0 +1,12 @@
+Require Import impboot.utils.Core.
+Require Import impboot.imp2asm.ImpToASMCodegen.
+Require Import impboot.imperative.Printing.
+Require Import impboot.imperative.ImpSyntax.
+Require Import impboot.parsing.Parser.
+Require Import impboot.assembly.ASMToString.
+
+Definition compiler (inp: string): string :=
+  let/d p := str2imp inp in
+  let/d asm := codegen p in
+  let/d str := asm2str asm in
+  str.
